full semantics

cakeSemantics/CakeAST.v
@@ -70,7 +70,65 @@ Inductive fptop : Type :=
 |  FP_Fma.
 
 Inductive op : Type :=
-  | Opapp : op.
+  | Opn : opn -> op
+  | Opb : opb -> op
+  | Opw : word_size -> opw -> op
+  | Shift : word_size -> shift -> nat -> op
+  | Equality : op
+  | OpFpCmp : fpcmp -> op
+  | OpFpUop : fpuop -> op
+  | OpFpBop : fpbop -> op
+  | OpFpTop : fptop -> op
+(* Function application *)
+  | Opapp : op
+  (* Reference operations *)
+  | Opassign : op
+  | Opref : op
+  | Opderef : op
+  (* Word8Array operations *)
+  | Aw8alloc : op
+  | Aw8sub : op
+  | Aw8length : op
+  | Aw8update : op
+  (* Word/integer conversions *)
+  | WordFromInt : word_size -> op
+  | WordToInt : word_size -> op
+  (* string/bytearray conversions *)
+  | CopyStrStr : op
+  | CopyStrAw8 : op
+  | CopyAw8Str : op
+  | CopyAw8Aw8 : op
+  (* Char operations *)
+  | Ord : op
+  | Chr : op
+  | Chopb : opb -> op
+  (* String operations *)
+  | Implode : op
+  | Explode : op
+  | Strsub : op
+  | Strlen : op
+  | Strcat : op
+  (* Vector operations *)
+  | VfromList : op
+  | Vsub : op
+  | Vlength : op
+  (* Array operations *)
+  | Aalloc : op
+  | AallocEmpty : op
+  | Asub : op
+  | Alength : op
+  | Aupdate : op
+  (* Unsafe array accesses *)
+  | Asub_unsafe : op
+  | Aupdate_unsafe : op
+  | Aw8sub_unsafe : op
+  | Aw8update_unsafe : op
+  (* List operations *)
+  | ListAppend : op
+  (* Configure the GC *)
+  | ConfigGC : op
+  (* Call a given foreign function *)
+  | FFI : string -> op.
 
 Inductive lop : Type :=
   | And : lop
@@ -94,6 +152,9 @@ Definition constr_id : Type :=
   option (ident modN conN).
 
 Inductive ast_t : Type :=
+  | Atvar : tvarN -> ast_t
+  | Atfun : ast_t -> ast_t -> ast_t
+  | Attup : list ast_t -> ast_t
   | Atapp : list ast_t -> ident modN typeN -> ast_t.
 Derive NoConfusion for ast_t.
 
@@ -107,11 +168,18 @@ Definition locs : Type := list nat.
 
 (* Expressions *)
 Inductive exp : Type :=
+  | ERaise : exp -> exp
+  | EHandle : exp -> list (pat * exp) -> exp
+  | ELit : lit -> exp
   | ECon : constr_id -> list exp -> exp
   | EVar : ident modN varN -> exp
   | EFun : varN -> exp -> exp
   | EApp : op -> list exp -> exp
+  | ELog : lop -> exp -> exp -> exp
+  | EIf  : exp -> exp -> exp -> exp
   | EMat : exp -> list (pat * exp) -> exp
+  | ELet : option varN -> exp -> exp -> exp
+  | ELetrec : list (varN * varN * exp) -> exp -> exp
   | ELannot : exp -> locs -> exp.
 Derive NoConfusion for exp.
 
@@ -124,7 +192,11 @@ Definition typeDef : Type :=
 Inductive dec : Type :=
   | Dlet : locs -> pat -> exp -> dec
   | Dletrec : locs -> list (varN * varN * exp) -> dec
-  | Dtype : locs -> typeDef -> dec.
+  | Dtype : locs -> typeDef -> dec
+  | Dtabbrev : locs -> list tvarN -> typeN -> ast_t -> dec
+  | Dexn : locs -> conN -> list ast_t -> dec
+  | Dmod : modN -> list dec -> dec
+  | Dlocal : list dec -> list dec -> dec.
 
 Fixpoint pat_bindings (p : pat) : list varN :=
   match p with
@@ -138,15 +210,22 @@ Fixpoint pat_bindings (p : pat) : list varN :=
 
 (** AST *)
 Fixpoint ast_t_rect' (P : ast_t -> Type)
-         (H1 : forall (l : list ast_t) (i : ident modN typeN), Forall'' P l -> P (Atapp l i))
+         (H1 : forall (s : tvarN), P (Atvar s))
+         (H2 : forall (a1 a2 : ast_t), P a1 -> P a2 -> P (Atfun a1 a2))
+         (H3 : forall (l : list ast_t), Forall'' P l -> P (Attup l))
+         (H4 : forall (l : list ast_t) (i : ident modN typeN), Forall'' P l -> P (Atapp l i))
          (a : ast_t) : P a :=
+  let fix loop (ls : list ast_t) :=
+      match ls with
+      | [] => Forall_nil'' ast_t P
+      | h::t => Forall_cons'' ast_t P h t (ast_t_rect' P H1 H2 H3 H4 h) (loop t)
+      end
+  in
   match a with
-  | Atapp l i => let fix F (ls : list ast_t) :=
-                   match ls with
-                   | [] => Forall_nil'' ast_t P
-                   | h::t => Forall_cons'' ast_t P h t (ast_t_rect' P H1 h) (F t)
-                   end
-               in H1 l i (F l)
+  | Atvar s => H1 s
+  | Atfun a1 a2 => H2 a1 a2 (ast_t_rect' P H1 H2 H3 H4 a1) (ast_t_rect' P H1 H2 H3 H4 a2)
+  | Attup l => H3 l (loop l)
+  | Atapp l i =>  H4 l i (loop l)
   end.
 
 Definition ast_t_ind' (P : ast_t -> Prop) := ast_t_rect' P.
@@ -186,16 +265,26 @@ Definition exp_rect_helper' (P : exp -> Type) (p : varN * varN * exp) : Type :=
   end.
 
 Fixpoint exp_rect' (P : exp -> Type)
-         (H1 : forall (o : constr_id) (l : list exp), Forall'' P l
-                                                                -> P (ECon o l))
-         (H2 : forall (i : ident modN varN), P (EVar i))
-         (H3 : forall (v : varN) (e : exp), P e -> P (EFun v e))
-         (H4 : forall (o : op) (l : list exp), Forall'' P l -> P (EApp o l))
-         (H5 : forall (e : exp), P e -> forall (l : list (pat * exp)), Forall'' (exp_rect_helper P) l
-                                                             -> P (EMat e l))
-         (H6 : forall (e : exp) (l : locs), P e -> P (ELannot e l))
+         (H  : forall (e' : exp), P e' -> P (ERaise e'))
+         (H0 : forall (e' : exp) (l : list (pat * exp)), P e' ->
+                                                    Forall'' (exp_rect_helper P) l ->
+                                                    P (EHandle e' l))
+         (H1 : forall (l : lit), P (ELit l))
+         (H2 : forall (o : constr_id) (l : list exp), Forall'' P l ->
+                                                 P (ECon o l))
+         (H3 : forall (i : ident modN varN), P (EVar i))
+         (H4 : forall (v : varN) (e : exp), P e -> P (EFun v e))
+         (H5 : forall (o : op) (l : list exp), Forall'' P l -> P (EApp o l))
+         (H6 : forall (lo : lop) (e1 e2 : exp), P e1 -> P e2 -> P (ELog lo e1 e2))
+         (H7 : forall (c t e : exp), P c -> P t -> P e -> P (EIf c t e))
+         (H8 : forall (e : exp), P e -> forall (l : list (pat * exp)), Forall'' (exp_rect_helper P) l ->
+                                                            P (EMat e l))
+         (H9 : forall (o : option varN) (e1 e2 : exp), P e1 -> P e2 -> P (ELet o e1 e2))
+         (H10 : forall (vve : list (varN * varN * exp)) (e : exp), Forall'' (exp_rect_helper' P) vve ->
+                                                   P e -> P (ELetrec vve e))
+         (H11 : forall (e : exp) (l : locs), P e -> P (ELannot e l))
          (e : exp) : P e :=
-  let exp_rect' := fun e' => exp_rect' P H1 H2 H3 H4 H5 H6 e' in
+  let exp_rect' := fun e' => exp_rect' P H H0 H1 H2 H3 H4 H5 H6 H7 H8 H9 H10 H11 e' in
   let fix loop (l : list exp) :=
       match l with
       | [] => Forall_nil'' exp P
@@ -215,12 +304,19 @@ Fixpoint exp_rect' (P : exp -> Type)
       end
   in
   match e with
-  | ECon o l  => H1 o l (loop l)
-  | EVar i    => H2 i
-  | EFun v e' => H3 v e' (exp_rect' e')
-  | EApp o l  => H4 o l (loop l)
-  | EMat e' l     => H5 e' (exp_rect' e') l (pair_loop l)
-  | ELannot e' l  => H6 e' l (exp_rect' e')
+  | ERaise e' => H e' (exp_rect' e')
+  | EHandle e' l => H0 e' l (exp_rect' e') (pair_loop l)
+  | ELit l => H1 l
+  | ECon o l  => H2 o l (loop l)
+  | EVar i    => H3 i
+  | EFun v e' => H4 v e' (exp_rect' e')
+  | EApp o l  => H5 o l (loop l)
+  | ELog lo e1 e2 => H6 lo e1 e2 (exp_rect' e1) (exp_rect' e2)
+  | EIf c t e => H7 c t e (exp_rect' c) (exp_rect' t) (exp_rect' e)
+  | EMat e' l     => H8 e' (exp_rect' e') l (pair_loop l)
+  | ELet o e1 e2  => H9 o e1 e2 (exp_rect' e1) (exp_rect' e2)
+  | ELetrec vve e => H10 vve e (trip_loop vve) (exp_rect' e)
+  | ELannot e' l  => H11 e' l (exp_rect' e')
   end.
 
 Definition exp_rec' (P : exp -> Set) := exp_rect' P.
@@ -235,19 +331,31 @@ Definition list_exp_rect_helper' (P : list exp -> Type) (p : varN * varN * exp) 
   match p with
   | (x, y, z) => P [z]
   end.
-Print list_rect.
 
 (** DEC *)
-
 Fixpoint dec_rect' (P : dec -> Type)
          (H1 : forall (l : locs) (p : pat) (e : exp), P (Dlet l p e))
          (H2 : forall (l : locs) (lv : list (varN * varN * exp)), P (Dletrec l lv))
          (H3 : forall (l : locs) (t : typeDef), P (Dtype l t))
+         (H4 : forall (l : locs) (tvs : list tvarN) (tn : typeN) (a : ast_t), P (Dtabbrev l tvs tn a))
+         (H5 : forall (l : locs) (cn : conN) (ls : list ast_t), P (Dexn l cn ls))
+         (H6 : forall (mn : modN) (ds : list dec), Forall'' P ds -> P (Dmod mn ds))
+         (H7 : forall (ds1 ds2 : list dec), Forall'' P ds1 -> Forall'' P ds2 -> P (Dlocal ds1 ds2))
          (d : dec) : P d :=
+  let fix loop (l : list dec) : Forall'' P l :=
+      match l with
+      | [] => Forall_nil'' _ _
+      | d'::l' => Forall_cons'' _ P d' l' (dec_rect' P H1 H2 H3 H4 H5 H6 H7 d') (loop l')
+      end
+  in
   match d with
   | Dlet l p e => H1 l p e
   | Dletrec l lv => H2 l lv
   | Dtype l t => H3 l t
+  | Dtabbrev l tvs tn a => H4 l tvs tn a
+  | Dexn l cn ls => H5 l cn ls
+  | Dmod mn ds => H6 mn ds (loop ds)
+  | Dlocal ds1 ds2 => H7 ds1 ds2 (loop ds1) (loop ds2)
   end.
 
 Definition dec_rec' (P : dec -> Set) := dec_rect' P.
@@ -298,10 +406,22 @@ Hint Resolve shift_eq_dec : DecidableEquality.
 
 Theorem op_eq_dec : forall (o0 o1 : op), {o0 = o1} + {o0 <> o1}.
 Proof.
-  destruct o0.
-  destruct o1.
-  left.
-  reflexivity.
+  decide equality.
+  - decide equality.
+  - decide equality.
+  - decide equality.
+  - decide equality.
+  - decide equality.
+  - decide equality.
+  - decide equality.
+  - decide equality.
+  - decide equality.
+  - decide equality.
+  - destruct f. destruct f0. left. reflexivity.
+  - decide equality.
+  - decide equality.
+  - decide equality.
+  - apply string_dec.
 Defined.
 
 Hint Resolve op_eq_dec : DecidableEquality.
@@ -312,26 +432,26 @@ Hint Resolve lop_eq_dec : DecidableEquality.
 
 Theorem ast_t_eq_dec : forall (a1 a2 : ast_t), {a1 = a2} + {a1 <> a2}.
 Proof.
-  intros.
-  apply (ast_t_rect' (fun a1 => forall a2, {a1 = a2} + {a1 <> a2})).
-  intros.
-  destruct a0.
-  destruct (ident_eq_dec _ _ string_dec string_dec i i0).
-  rewrite e.
-  generalize dependent l0.
-  induction X;
-  destruct l0;
-    try (left; congruence);
-    try (right; congruence).
-  destruct (p a).
-  destruct (IHX l0).
-  inv e1.
-  subst.
-  left; congruence.
-  subst.
-  right; congruence.
-  right; congruence.
-  right; congruence.
+  decide equality.
+  - apply string_dec.
+  - generalize dependent l0. induction X; destruct l0.
+    left; reflexivity.
+    right; congruence.
+    right; congruence.
+    destruct (IHX l0). destruct (p a). subst.
+    left; reflexivity.
+    right; congruence.
+    right; congruence.
+  - apply ident_eq_dec; apply string_dec.
+  - generalize dependent l0. induction X; destruct l0.
+    left; reflexivity.
+    right; congruence.
+    right; congruence.
+    destruct (IHX l0).
+    destruct (p a). subst.
+    left; reflexivity.
+    right; congruence.
+    right. congruence.
 Defined.
 Hint Resolve ast_t_eq_dec : DecidableEquality.
 
@@ -375,6 +495,18 @@ Ltac tryl := try (left; congruence).
 Theorem exp_eq_dec : forall (e0 e1 : exp), {e0 = e1} + {e0 <> e1}.
 Proof.
   induction e0 using exp_rect'; destruct e1; try (right; congruence).
+  - destruct (IHe0 e1); tryl; tryr.
+  - generalize dependent l0.
+    induction X; destruct l0; destruct (IHe0 e1); tryl; tryr.
+    destruct x. destruct p0.
+    simpl in *. destruct (p e3).
+    destruct (pat_eq_dec p1 p0).
+    destruct (IHX l0).
+    tryl.
+    tryr.
+    tryr.
+    tryr.
+  - destruct (lit_eq_dec l l0); tryl; tryr.
   - destruct (constr_id_eq_dec o c); try (right; congruence).
     generalize dependent l0.
     induction X; destruct l0; try (right; congruence).
@@ -396,6 +528,16 @@ Proof.
     destruct (p e0); tryr.
     inv e1; subst.
     tryl.
+  - destruct (IHe0_1 e1_1); tryr.
+    destruct (IHe0_2 e1_2); tryr.
+    destruct (lop_eq_dec lo l); tryl; tryr.
+  - destruct (IHe0_1 e1_1).
+    destruct (IHe0_2 e1_2).
+    destruct (IHe0_3 e1_3).
+    subst. tryl.
+    tryr.
+    tryr.
+    tryr.
   - generalize dependent l0.
     destruct (IHe0 e1); tryr.
     induction X; destruct l0; tryr.
@@ -407,6 +549,17 @@ Proof.
     destruct (p e4); tryr.
     destruct (pat_eq_dec p1 p0); tryr.
     subst; inv e2; tryl.
+  - destruct (option_eq_dec _ string_dec o o0); tryr.
+    destruct (IHe0_1 e1_1); tryr.
+    destruct (IHe0_2 e1_2); tryl; tryr.
+  - destruct (IHe0 e1); tryr.
+    generalize dependent l. induction X; intro l0; destruct l0; tryl; tryr.
+    destruct x. destruct p1. destruct p0. destruct p0.
+    simpl in p.
+    destruct (IHX l0); tryr.
+    destruct (string_dec v v1); tryr.
+    destruct (string_dec v0 v2); tryr.
+    destruct (p e3); tryl; tryr.
   - destruct (locs_eq_dec l l0); tryr.
     destruct (IHe0 e1); tryr.
     subst; tryl.
@@ -414,11 +567,36 @@ Defined.
 Hint Resolve exp_eq_dec : DecidableEquality.
 Instance EqDec_exp : EqDec exp := exp_eq_dec.
 
-Print EqDec_exp.
-
 Theorem dec_eq_dec : forall (d0 d1 : dec), {d0 = d1} + {d0 <> d1}.
 Proof.
   decide equality; try (auto with DecidableEquality).
+  - generalize dependent l. induction X; intros l'; destruct l'.
+    left; reflexivity.
+    right; congruence.
+    right; congruence.
+    destruct (IHX l').
+    destruct (p d).
+    subst; left; reflexivity.
+    right; congruence.
+    right; congruence.
+  - generalize dependent l0. induction X0; intros l'; destruct l'.
+    left; reflexivity.
+    right; congruence.
+    right; congruence.
+    destruct (IHX0 l').
+    destruct (p d).
+    subst; left; reflexivity.
+    right; congruence.
+    right; congruence.
+  - generalize dependent l. induction X; intros l'; destruct l'.
+    left; reflexivity.
+    right; congruence.
+    right; congruence.
+    destruct (IHX l').
+    destruct (p d).
+    subst; left; reflexivity.
+    right; congruence.
+    right; congruence.
 Defined.
 Hint Resolve dec_eq_dec : DecidableEquality.
 
