cakeSemantics/FreeVars.v
@@ -45,28 +45,60 @@ Fixpoint free_vars (e : exp) : list (ident modN varN) :=
           end
       in
       match e with
-      (* | ERaise e' => free_vars_helper e' bl *)
-      (* | EHandle e' pes => free_vars_helper e' bl ++ pattern_match_free_vars pes bl *)
-      (* | ELit _ => [] *)
+      | ERaise e' => free_vars_helper e' bl
+      | EHandle e' pes => free_vars_helper e' bl ++ pattern_match_free_vars pes bl
+      | ELit _ => []
       | ECon cid es => exp_list_free_vars es bl
       | EVar id => if in_dec (fun i i' => ident_eq_dec _ _ string_dec string_dec i i' ) id bl
                   then []
                   else [id]
       | EFun var_name e' => free_vars_helper e' ((Short var_name)::bl)
       | EApp o es => exp_list_free_vars es bl
-      (* | ELog o e1 e2 => free_vars_helper e1 bl ++ free_vars_helper e2 bl *)
-      (* | EIf c t f => free_vars_helper c bl ++ free_vars_helper t bl ++ free_vars_helper f bl *)
+      | ELog o e1 e2 => free_vars_helper e1 bl ++ free_vars_helper e2 bl
+      | EIf c t f => free_vars_helper c bl ++ free_vars_helper t bl ++ free_vars_helper f bl
       | EMat e' pes => free_vars_helper e' bl ++ pattern_match_free_vars pes bl
-      (* | ELet opt_var_name e1 e2 => match opt_var_name with *)
-      (*                             | None => free_vars_helper e1 bl ++ free_vars_helper e2 bl *)
-      (*                             | Some name => free_vars_helper e1 bl ++ free_vars_helper e2 ((Short name)::bl) *)
-      (*                             end *)
-      (* | ELetrec vves e' => free_vars_helper e' (map (fun x => Short (fst (fst x))) vves ++ bl) ++ vvexp_list_free_vars vves bl *)
+      | ELet opt_var_name e1 e2 => match opt_var_name with
+                                  | None => free_vars_helper e1 bl ++ free_vars_helper e2 bl
+                                  | Some name => free_vars_helper e1 bl ++ free_vars_helper e2 ((Short name)::bl)
+                                  end
+      | ELetrec vves e' => free_vars_helper e' (map (fun x => Short (fst (fst x))) vves ++ bl) ++ vvexp_list_free_vars vves bl
       (* | ETannot e' _ => free_vars_helper e' bl *)
       | ELannot e' _ => free_vars_helper e' bl
       end
   in
   free_vars_helper e [].
+
+Fixpoint pat_used_cons (p:pat) : list (ident modN varN) :=
+  match p with
+  (* | Pany | Plit _ => [] *)
+  | Pvar v => []
+  | Pcon cid pl => match cid with
+                  | None => concat (map pat_used_cons pl)
+                  | Some id => id :: (concat (map pat_used_cons pl))
+                  end
+  (* | Pref p' | Ptannot p' _ => pattern_vars p' *)
+  end.
+
+Fixpoint used_cons (e : exp) : list (ident modN varN) :=
+  match e with
+  | ERaise e' => used_cons e'
+  | EHandle e' pes => used_cons e' ++ (concat (map (fun x => pat_used_cons (fst x) ++ used_cons (snd x)) pes))
+  | ELit _ => []
+  | ECon cid es => match cid with
+                  | None => (concat (map used_cons es))
+                  | Some id => id :: (concat (map used_cons es))
+                  end
+  | EVar id => []
+  | EFun var_name e' => used_cons e'
+  | EApp o es => concat (map used_cons es)
+  | ELog o e1 e2 => used_cons e1 ++ used_cons e2
+  | EIf c t f => used_cons c ++ used_cons t ++ used_cons f
+  | EMat e' pes => used_cons e' ++ (concat (map (fun x => pat_used_cons (fst x) ++ used_cons (snd x)) pes))
+  | ELet opt_var_name e1 e2 => used_cons e1 ++ used_cons e2
+  | ELetrec vves e' => used_cons e' ++ (concat (map (fun x => used_cons (snd x)) vves))
+  (* | ETannot e' _ => free_vars_helper e' bl *)
+  | ELannot e' _ => used_cons e'
+  end.
 
 (* Shell of a function that may need be defined in the future *)
 (* Fixpoint free_vars_dec (d : dec) : list (ident modN varN) := *)
